src/TacPackIL.v
@@ -206,7 +206,7 @@ Module ILAlgoTypes <: AlgoTypes SEP BedrockCoreEnv.
       Require Provers.
       (** Test **)
       Goal TypedPackage.
-        build_prover_pack provers.TransitivityProver.TransitivityProver ltac:(fun x => refine x).
+        build_prover_pack provers.ReflexivityProver.ReflexivityProver ltac:(fun x => refine x).
       Defined.
     End ProverPackTest.
 
@@ -440,14 +440,14 @@ Ltac opaque_pack pack :=
   end.
 
 Goal TypedPackage.
-  build_prover_pack provers.TransitivityProver.TransitivityProver ltac:(fun x => 
+  build_prover_pack provers.ReflexivityProver.ReflexivityProver ltac:(fun x => 
     build_mem_pack (MEVAL.Default.package bedrock_types_r (tvType 0) (tvType 1) (tvType 0) (tvType 0) IL_mem_satisfies IL_ReadWord IL_WriteWord) ltac:(fun y =>   
     glue_pack x y ltac:(opaque_pack))).
 Qed.
 
 (*
 Goal TypedPackage bedrock_types_r (tvType 0) (tvType 1) IL_mem_satisfies IL_ReadWord IL_WriteWord.
-  build_prover_pack Provers.TransitivityProver ltac:(fun x => 
+  build_prover_pack Provers.ReflexivityProver ltac:(fun x => 
     build_mem_pack (MEVAL.Default.package bedrock_types_r (tvType 0) (tvType 1) (tvType 0) (tvType 0) IL_mem_satisfies IL_ReadWord IL_WriteWord) ltac:(fun y =>   
       idtac "1" ;
     glue_packs (x, y, y) ltac:(fun v => exact v))).
